utp_rad_healthy.thy
@@ -4,21 +4,25 @@ theory utp_rad_healthy
   imports utp_rad_bridge
 begin
 
-subsection \<open>Trace extension (Paper Definitions 27 and 28)\<close>
+subsection \<open>RA1: Trace extension\<close>
 
+(* Paper Definition 27. *)
 definition rad_trace_extensions :: "'e rad_state \<Rightarrow> 'e rad_state set" where
 "rad_trace_extensions x =
   {z. rad_state.tr\<^sub>v x \<le> rad_state.tr\<^sub>v z}"
 
+(* Paper Definition 28. *)
+(* RA1(P)(x, A) = P(x, rad_trace_extension(x) \<inter> A) ∧ A' \<noteq> \<emptyset> *)
 definition RA1 ::
-  "'e reactive_angelic_design \<Rightarrow> 'e reactive_angelic_design"
-where
+  "'e reactive_angelic_design \<Rightarrow> 'e reactive_angelic_design" where
 "RA1 P = (\<lambda> (x, y).
-  let s0 = get\<^bsub>s\<^esub> (get\<^bsub>\<^bold>v\<^sub>D\<^esub> x);
-      A = get\<^bsub>ac\<^esub> (get\<^bsub>\<^bold>v\<^sub>D\<^esub> y);
+  let x_state = des_vars.more x;
+      y_choices = des_vars.more y;
+      s0 = astate.s\<^sub>v x_state;
+      A = achoices.ac\<^sub>v y_choices;
       A' = rad_trace_extensions s0 \<inter> A;
-      y' = put\<^bsub>\<^bold>v\<^sub>D\<^esub> y
-        (put\<^bsub>ac\<^esub> (get\<^bsub>\<^bold>v\<^sub>D\<^esub> y) A')
+      y_choices' = achoices.ac\<^sub>v_update (\<lambda>_. A') y_choices;
+      y' = des_vars.more_update (\<lambda>_. y_choices') y
   in P (x, y') \<and> A' \<noteq> {})"
 
 lemma RA1_idem: "RA1 (RA1 P) = RA1 P"
@@ -31,83 +35,232 @@ lemma RA1_mono:
   "P \<sqsubseteq> Q \<Longrightarrow> RA1 P \<sqsubseteq> RA1 Q"
   by (auto simp add: RA1_def pred_refine_iff Let_def split: prod.splits)
 
-lemma RA1_Monotonic [closure]: "Monotonic RA1"
+lemma RA1_Monotonic [closure]:
+  "Monotonic RA1"
   by (rule MonotonicI, rule RA1_mono)
 
-subsection \<open>Trace-history independence (Paper Definition 29)\<close>
+(* Paper Theorem 9. *)
+lemma RA1_A0: "RA1 (A0 P) = RA1 P"
+  apply (simp add: RA1_def A0_def ac_non_empty_def fun_eq_iff)
+  apply (pred_auto)
+  apply (simp_all add: Let_def)
+  done
 
+(* Paper Example 11.  PBMH_ades is the lifting of the paper's PBMH through
+   the outer design record. *)
+definition rad_ac_empty :: "'e reactive_angelic_design" where
+"rad_ac_empty = (\<lambda> (x, y).
+  achoices.ac\<^sub>v (des_vars.more y) = {})"
+
+lemma PBMH_ades_ac_empty [simp]:
+  "PBMH_ades rad_ac_empty = true"
+  by (simp add: PBMH_ades_def rad_ac_empty_def; pred_auto)
+
+lemma RA1_ac_empty [simp]:
+  "RA1 rad_ac_empty = false"
+  by (simp add: RA1_def rad_ac_empty_def fun_eq_iff; pred_auto)
+
+lemma RA1_PBMH_ades_ac_empty:
+  "RA1 (PBMH_ades rad_ac_empty) = RA1 true"
+  by simp
+
+lemma PBMH_ades_RA1_ac_empty:
+  "PBMH_ades (RA1 rad_ac_empty) = false"
+  by (simp add: PBMH_ades_def; pred_auto)
+
+lemma RA1_PBMH_ades_not_commute:
+  "RA1 (PBMH_ades rad_ac_empty) \<noteq>
+   PBMH_ades (RA1 rad_ac_empty)"
+  by (simp only: RA1_PBMH_ades_ac_empty PBMH_ades_RA1_ac_empty;
+      simp add: RA1_def rad_trace_extensions_def fun_eq_iff; pred_auto)
+
+subsection \<open>RA2: Trace-history independence\<close>
+
+(* s \<oplus> {tr ↦ []} *)
 definition rad_zero_trace :: "'e rad_state \<Rightarrow> 'e rad_state" where
-"rad_zero_trace x = put\<^bsub>rad_state.tr\<^esub> x []"
+"rad_zero_trace s\<^sub>0 =
+  rad_state.tr\<^sub>v_update (\<lambda>_. []) s\<^sub>0"
 
+(* z \<oplus> {tr ↦ z.tr - s.tr} *)
 definition rad_trace_difference ::
-  "'e rad_state \<Rightarrow> 'e rad_state \<Rightarrow> 'e rad_state"
-where
-"rad_trace_difference x z =
-  put\<^bsub>rad_state.tr\<^esub> z (rad_state.tr\<^sub>v z - rad_state.tr\<^sub>v x)"
+  "'e rad_state \<Rightarrow> 'e rad_state \<Rightarrow> 'e rad_state" where
+"rad_trace_difference s\<^sub>0 z =
+  rad_state.tr\<^sub>v_update
+    (\<lambda>_. rad_state.tr\<^sub>v z - rad_state.tr\<^sub>v s\<^sub>0) z"
 
+(* { z[(z.tr-s.tr) / tr] | z \<in> ac' ∧ s.tr \<le> z.tr } *)
 definition rad_normalise_choices ::
-  "'e rad_state \<Rightarrow> 'e rad_state set \<Rightarrow> 'e rad_state set"
-where
-"rad_normalise_choices x choices =
-  {rad_trace_difference x z | z.
-    z \<in> choices \<and> rad_state.tr\<^sub>v x \<le> rad_state.tr\<^sub>v z}"
+  "'e rad_state \<Rightarrow> 'e rad_state set \<Rightarrow> 'e rad_state set" where
+"rad_normalise_choices s\<^sub>0 ac' =
+  {rad_trace_difference s\<^sub>0 z | z.
+    z \<in> ac' \<and>
+    rad_state.tr\<^sub>v s\<^sub>0 \<le> rad_state.tr\<^sub>v z}"
 
+(* Paper Definition 29. *)
+(* RA2(P)(s,ac') = P(s[[]/tr], rad_normalise_choices(s, ac')) *)
 definition RA2 ::
   "'e reactive_angelic_design \<Rightarrow> 'e reactive_angelic_design"
-where
-"RA2 P = (\<lambda> (x, y).
-  let s0 = get\<^bsub>s\<^esub> (get\<^bsub>\<^bold>v\<^sub>D\<^esub> x);
-      A = get\<^bsub>ac\<^esub> (get\<^bsub>\<^bold>v\<^sub>D\<^esub> y);
-      x' = put\<^bsub>\<^bold>v\<^sub>D\<^esub> x
-        (put\<^bsub>s\<^esub> (get\<^bsub>\<^bold>v\<^sub>D\<^esub> x) (rad_zero_trace s0));
-      y' = put\<^bsub>\<^bold>v\<^sub>D\<^esub> y
-        (put\<^bsub>ac\<^esub> (get\<^bsub>\<^bold>v\<^sub>D\<^esub> y)
-          (rad_normalise_choices s0 A))
+where "RA2 P = (\<lambda> (x, y).
+  let x_state = des_vars.more x;
+      y_choices = des_vars.more y;
+      s\<^sub>0 = astate.s\<^sub>v x_state;
+      ac' = achoices.ac\<^sub>v y_choices;
+      ac'' = rad_normalise_choices s\<^sub>0 ac';
+      x_state' = astate.s\<^sub>v_update
+        (\<lambda>_. rad_zero_trace s\<^sub>0) x_state;
+      y_choices' = achoices.ac\<^sub>v_update (\<lambda>_. ac'') y_choices;
+      x' = des_vars.more_update (\<lambda>_. x_state') x;
+      y' = des_vars.more_update (\<lambda>_. y_choices') y
   in P (x', y'))"
+
+lemma RA2_idem: "RA2 (RA2 P) = RA2 P"
+  by (simp add: RA2_def rad_zero_trace_def rad_normalise_choices_def
+      rad_trace_difference_def fun_eq_iff)
+
+lemma RA2_Idempotent: "Idempotent RA2"
+  by (simp add: Idempotent_def RA2_idem)
+
+lemma rad_normalise_choices_extensions:
+  "rad_normalise_choices s0 (rad_trace_extensions s0 \<inter> choices) =
+   rad_normalise_choices s0 choices"
+  by (auto simp add: rad_normalise_choices_def rad_trace_extensions_def)
+
+lemma rad_normalise_choices_nonempty:
+  "rad_normalise_choices s0 choices \<noteq> {} \<longleftrightarrow>
+   rad_trace_extensions s0 \<inter> choices \<noteq> {}"
+  by (auto simp add: rad_normalise_choices_def rad_trace_extensions_def)
+
+lemma rad_zero_trace_extensions:
+  "rad_trace_extensions (rad_zero_trace s0) \<inter>
+   rad_normalise_choices s0 choices =
+   rad_normalise_choices s0 choices"
+  by (auto simp add: rad_trace_extensions_def rad_zero_trace_def
+      rad_normalise_choices_def rad_trace_difference_def)
+
+lemma rad_zero_trace_in_normalise:
+  "rad_zero_trace s0 \<in> rad_normalise_choices s0 choices \<longleftrightarrow>
+   s0 \<in> choices"
+  apply (auto simp add: rad_zero_trace_def rad_normalise_choices_def
+      rad_trace_difference_def)
+  subgoal for z
+    apply (cases s0; cases z)
+    apply (simp_all add: less_eq_list_def minus_list_def)
+    apply (metis prefix_length_eq prefix_imp_length_lteq order_antisym)
+    done
+  subgoal
+    by (rule exI[where x=s0], simp)
+  done
+
+(* Thesis T.5.2.10. *)
+lemma RA1_RA2_commute:
+  "RA1 (RA2 P) = RA2 (RA1 P)"
+  by (simp add: RA1_def RA2_def fun_eq_iff
+      rad_normalise_choices_extensions rad_normalise_choices_nonempty
+      rad_zero_trace_extensions Let_def)
 
 lemma RA2_mono:
   "P \<sqsubseteq> Q \<Longrightarrow> RA2 P \<sqsubseteq> RA2 Q"
   by (auto simp add: RA2_def pred_refine_iff Let_def split: prod.splits)
 
-lemma RA2_Monotonic [closure]: "Monotonic RA2"
+lemma RA2_Monotonic [closure]:
+  "Monotonic RA2"
   by (rule MonotonicI, rule RA2_mono)
 
-subsection \<open>Reactive identity and waiting (Paper Definitions 30 and 31)\<close>
+subsection \<open>RA3. Reactive identity and waiting\<close>
 
+(* Paper Definition 30. Rac identity *)
 definition II_Rac :: "'e reactive_angelic_design" where
 "II_Rac = (\<lambda> (x, y).
-  let s0 = get\<^bsub>s\<^esub> (get\<^bsub>\<^bold>v\<^sub>D\<^esub> x);
-      A = get\<^bsub>ac\<^esub> (get\<^bsub>\<^bold>v\<^sub>D\<^esub> y)
-  in RA1 (\<lambda> (x, y). \<not> ok\<^sub>v x) (x, y) \<or> (ok\<^sub>v x \<and> s0 \<in> A))"
+  let s0 = astate.s\<^sub>v (des_vars.more x);
+      A = achoices.ac\<^sub>v (des_vars.more y)
+  in RA1 (\<lambda> (x, y). \<not> ok\<^sub>v x) (x, y) \<or> (ok\<^sub>v y \<and> s0 \<in> A))"
 
+(* Thesis T.G.3.1--T.G.3.4. *)
+lemma RA1_II_Rac:
+  "RA1 II_Rac = II_Rac"
+  apply (simp only: RA1_def II_Rac_def fun_eq_iff)
+  apply (simp add: Let_def rad_trace_extensions_def
+      des_vars.ok_def des_vars.more\<^sub>L_def)
+  apply blast
+  done
+
+lemma RA2_II_Rac:
+  "RA2 II_Rac = II_Rac"
+  apply (simp only: RA2_def II_Rac_def fun_eq_iff)
+  apply (simp add: Let_def RA1_def rad_zero_trace_extensions
+      rad_normalise_choices_nonempty rad_zero_trace_in_normalise
+      des_vars.ok_def des_vars.more\<^sub>L_def)
+  done
+
+abbreviation rad_wait_lens where
+"rad_wait_lens \<equiv>
+  rad_state.wait ;\<^sub>L astate.s ;\<^sub>L des_vars.more\<^sub>L"
+
+(* Paper Definition 31. *)
 definition RA3 ::
-  "'e reactive_angelic_design \<Rightarrow> 'e reactive_angelic_design"
-where
-"RA3 P = (\<lambda> (x, y).
-  if rad_state.wait\<^sub>v
-      (get\<^bsub>s\<^esub> (get\<^bsub>\<^bold>v\<^sub>D\<^esub> x))
-  then II_Rac (x, y)
-  else P (x, y))"
+  "'e reactive_angelic_design \<Rightarrow> 'e reactive_angelic_design" where
+"RA3 P = (II_Rac \<triangleleft> $rad_wait_lens\<^sup>< \<triangleright> P)"
+
+lemma RA1_wait_cond:
+  "RA1 (P \<triangleleft> $rad_wait_lens\<^sup>< \<triangleright> Q) =
+   (RA1 P \<triangleleft> $rad_wait_lens\<^sup>< \<triangleright> RA1 Q)"
+  by (simp add: RA1_def expr_if_def fun_eq_iff Let_def lens_defs
+      rad_state.wait_def astate.s_def des_vars.more\<^sub>L_def)
+
+lemma RA2_wait_cond:
+  "RA2 (P \<triangleleft> $rad_wait_lens\<^sup>< \<triangleright> Q) =
+   (RA2 P \<triangleleft> $rad_wait_lens\<^sup>< \<triangleright> RA2 Q)"
+  by (simp add: RA2_def expr_if_def fun_eq_iff Let_def lens_defs
+      rad_zero_trace_def rad_state.wait_def astate.s_def
+      des_vars.more\<^sub>L_def)
+
+lemma RA3_idem:
+  "RA3 (RA3 P) = RA3 P"
+  by (simp add: RA3_def)
+
+lemma RA3_Idempotent:
+  "Idempotent RA3"
+  by (simp add: Idempotent_def RA3_idem)
+
+(* Thesis T.5.2.16--T.5.2.17. *)
+lemma RA1_RA3_commute:
+  "RA1 (RA3 P) = RA3 (RA1 P)"
+  by (simp add: RA3_def RA1_wait_cond RA1_II_Rac)
+
+lemma RA2_RA3_commute:
+  "RA2 (RA3 P) = RA3 (RA2 P)"
+  by (simp add: RA3_def RA2_wait_cond RA2_II_Rac)
 
 lemma RA3_mono:
   "P \<sqsubseteq> Q \<Longrightarrow> RA3 P \<sqsubseteq> RA3 Q"
   by (simp add: RA3_def, pred_auto)
 
-lemma RA3_Monotonic [closure]: "Monotonic RA3"
+lemma RA3_Monotonic [closure]:
+  "Monotonic RA3"
   by (rule MonotonicI, rule RA3_mono)
 
-subsection \<open>Reactive angelic healthiness (Paper Definition 32)\<close>
+subsection \<open>RA\<close>
 
+(* Paper Definition 32. *)
 definition RA ::
-  "'e reactive_angelic_design \<Rightarrow> 'e reactive_angelic_design"
-where
+  "'e reactive_angelic_design \<Rightarrow> 'e reactive_angelic_design" where
 "RA = RA1 \<circ> RA2 \<circ> RA3"
+
+lemma RA_idem:
+  "RA (RA P) = RA P"
+  by (simp add: RA_def RA1_RA2_commute RA1_RA3_commute
+      RA2_RA3_commute RA1_idem RA2_idem RA3_idem)
+
+lemma RA_Idempotent:
+  "Idempotent RA"
+  by (simp add: Idempotent_def RA_idem)
 
 lemma RA_mono:
   "P \<sqsubseteq> Q \<Longrightarrow> RA P \<sqsubseteq> RA Q"
   by (simp add: RA_def RA1_mono RA2_mono RA3_mono)
 
-lemma RA_Monotonic [closure]: "Monotonic RA"
+lemma RA_Monotonic [closure]:
+  "Monotonic RA"
   unfolding RA_def
   by (intro Monotonic_comp RA1_Monotonic RA2_Monotonic RA3_Monotonic)
 
